src/coq/TopLevelRefinements.v
@@ -1,0 +1,22 @@
+From ITree Require Import
+     ITree
+     ITreeFacts
+     Events.StateFacts
+     Eq.Eq.
+
+From Vellvm Require Import
+     Memory
+     Refinement
+     Environment
+     TopLevel
+     LLVMAst
+     Handlers.Stack.
+
+Module R := Refinement.Make(Memory.A)(IO)(TopLevelEnv).
+Import R.
+Import TopLevelEnv.
+
+(* Do I want to restrict this? *)
+Lemma refine_01: forall t1 t2,
+    refine_L0 t1 t2 -> refine_L1 (build_L1 t1) (build_L1 t2).
+Abort.
