src/coq/Environment.v
@@ -1,0 +1,6 @@
+Module Type Environment.
+  Parameter local_env  : Type.
+  Parameter global_env : Type.
+  Parameter stack      : Type.
+  Parameter memory     : Type.
+End Environment.
